List

Learn.List.fst
@@ -4,6 +4,7 @@ open FStar.Calc
 open FStar.Classical.Sugar
 open FStar.List.Pure
 
+module U = Learn.Util
 module T  = FStar.Tactics
 module Cl = FStar.Classical
 
@@ -14,7 +15,7 @@ let rec append_index (#a:Type) (l1 l2 : list a) (i : nat{i < length l1 + length 
     | _ :: tl -> if i = 0 then () else append_index tl l2 (i-1)
 
 (* [reverse] *)
-
+(* TODO: already defined as [rev'] *)
 let rec reverse (#a:Type) (l : list a) : list a =
   match l with
   | [] -> []
@@ -125,7 +126,20 @@ let rec for_all_opairsP (#a : Type) (f : a -> a -> prop) (l : list a) : prop
     | [] -> True
     | hd :: tl -> for_allP (f hd) tl /\ for_all_opairsP f tl
 
-let iff (a b : Type) : Type = (a -> b) & (b -> a)
+(*
+let iffI (d0 : T.term -> T.Tac unit) (d1 : T.term -> T.Tac unit) : T.Tac unit =
+  T.(split (); iseq [(fun () -> let h = implies_intro () in d0 h);
+                     (fun () -> let h = implies_intro () in d1 h)])
+
+let test_iff (a : Type) (p : a -> Type) : GTot (squash ((forall x . p x) <==> (forall x . p x))) =
+  _ by T.(iffI (fun h -> let x  = forall_intro () in
+                      let h' = instantiate h x in
+                      hyp h')
+               (fun _ -> smt ()))
+
+let test_impl (p : nat -> Type) (l : p 0 -> squash (p 1)) : GTot ((squash (p 0 ==> p 1))) =
+  _ by T.(let h = implies_intro () in apply (quote l); hyp h)
+*)
 
 let rec for_all_opairsP_index (#a : Type) (f : a -> a -> prop) (l : list a)
   : Lemma (for_all_opairsP f l
@@ -133,13 +147,6 @@ let rec for_all_opairsP_index (#a : Type) (f : a -> a -> prop) (l : list a)
   = match l with
     | [] -> ()
     | hd :: tl ->
-         (*let lem0 :
-           ((j:nat{j < length tl} -> f hd (index tl j))
-             & ((i:nat{i < length tl}) -> j:nat{j < length tl} -> squash (i < j) -> f (index tl i) (index tl j)))
-           ->
-           (i:nat{i < length l} -> j:nat{j < length l} -> squash (i < j) -> f (index l i) (index l j))
-           = fun (h0, h1) i j lt -> if i = 0 then h0 (j-1) else h1 (i-1) (j-1) ()
-         in*)
          introduce
               (forall (j:nat{j < length tl}). f hd (index tl j))
            /\ (forall (i j : (x:nat{x < length tl})). i < j ==> f (index tl i) (index tl j))
@@ -154,29 +161,6 @@ let rec for_all_opairsP_index (#a : Type) (f : a -> a -> prop) (l : list a)
               else eliminate forall (i j : (x:nat{x < length tl})). i < j ==> f (index tl i) (index tl j)
                         with (i-1) (j-1)
          ;
-       (* let lem1 :
-           (i:nat{i < length l} -> j:nat{j < length l} -> squash (i < j) -> f (index l i) (index l j))
-           ->
-           ((j:nat{j < length tl} -> f hd (index tl j))
-             & ((i:nat{i < length tl}) -> j:nat{j < length tl} -> squash (i < j) -> f (index tl i) (index tl j)))
-           = fun h -> (fun (j:nat{j<length tl}) -> h 0 (j+1) ()),
-                   (fun (i:nat{i<length tl}) (j:nat{j<length tl}) lt -> h (i+1) (j+1) ())
-         in*)
-       (*
-         introduce
-              (forall (i j : (x:nat{x < length l})). i < j ==> f (index l i) (index l j))
-           ==>
-              (forall (j:nat{j < length tl}). f hd (index tl j))
-           /\ (forall (i j : (x:nat{x < length tl})). i < j ==> f (index tl i) (index tl j))
-         with h. introduce (forall (j:nat{j < length tl}). f hd (index tl j))
-                        /\ (forall (i j : (x:nat{x < length tl})). i < j ==> f (index tl i) (index tl j))
-           with (introduce forall (j:nat{j < length tl}). _
-                 with eliminate forall i j. i < j ==> f (index l i) (index l j)
-                           with 0 (j+1))
-            and (introduce forall (i j : (x:nat{x < length tl})). _
-                 with eliminate forall i j. i < j ==> f (index l i) (index l j)
-                           with (i+1) (j+1));*)
-
          calc (<==>) {
            for_all_opairsP f (hd :: tl);
          <==> {}
@@ -184,7 +168,7 @@ let rec for_all_opairsP_index (#a : Type) (f : a -> a -> prop) (l : list a)
          <==> {for_allP_index (f hd) tl; for_all_opairsP_index f tl}
               (forall (j:nat{j < length tl}). f hd (index tl j))
            /\ (forall (i j : (x:nat{x < length tl})). i < j ==> f (index tl i) (index tl j));
-         <==> {}
+         <==> { }
               (forall (j:nat{j < length tl}). f (index l 0) (index l (j+1)))
            /\ (forall (i j : (x:nat{x < length tl})). i < j ==> f (index l (i+1)) (index l (j+1)));
          <==> {}
@@ -254,3 +238,141 @@ let rec map_insert (#a #b : Type) (f : a -> b) (i : nat) (x : a) (l : list a)
           (decreases i)
   = if i = 0 then ()
     else map_insert f (i - 1) x (tail l)
+
+(* [set] *)
+
+let rec set (#a : Type) (i : nat) (x : a) (l : list a)
+  : Pure (list a) (requires i < length l) (ensures fun r -> length r = length l)
+         (decreases i)
+  = let hd :: tl = l in
+    if i = 0 then x :: tl
+    else hd :: set (i - 1) x tl
+
+(* [map_index] *)
+
+let rec map_index (#a : Type) (i : nat) (f : a -> a) (l : list a)
+  : Pure (list a) (requires i < length l) (ensures fun r -> length r = length l)
+         (decreases i)
+  = let hd :: tl = l in
+    if i = 0 then f hd :: tl
+    else hd :: map_index (i - 1) f tl
+
+let rec set_is_map_index (#a : Type) (i : nat) (x : a) (l : list a)
+  : Lemma (requires  i < length l)
+          (ensures   set i x l == map_index i (fun _ -> x) l)
+          (decreases i)
+  = if i = 0 then () else set_is_map_index (i-1) x (tail l)
+
+(* [splitAt] *)
+
+let rec lemma_splitAt_append (#a:Type) (n:nat) (l:list a) :
+  Lemma (ensures (let l1, l2 = splitAt n l in append l1 l2 == l)) =
+  match n with
+  | 0 -> ()
+  | _ ->
+    match l with
+    | [] -> ()
+    | x :: xs -> lemma_splitAt_append (n-1) xs
+
+(* [permutation] *)
+
+noeq type permutation_t (#a : Type) : list a -> list a -> Type =
+  | Perm_swap : l0 : list a -> x : a -> y : a -> l1 : list a ->
+              permutation_t (l0 @ x :: y :: l1) (l0 @ y :: x :: l1)
+  | Perm_refl  : l : list a -> permutation_t l l
+  | Perm_trans : l0 : list a -> l1 : list a -> l2 : list a ->
+              permutation_t l0 l1 -> permutation_t l1 l2 ->
+              permutation_t l0 l2
+
+type permutation #a l0 l1 = squash (permutation_t #a l0 l1)
+
+module Mnd = FStar.Algebra.Monoid
+
+let append_monoid (a : Type) : Mnd.monoid (list a) =
+  U.assert_by (Mnd.right_unitality_lemma (list a) [] (append #a) /\ True)
+    (fun () -> assert (forall (l : list a) . l @ [] == l));
+  assert (Mnd.left_unitality_lemma (list a) [] (append #a));
+  U.assert_by (Mnd.associativity_lemma (list a) (append #a) /\ True)
+    (fun () -> assert (Mnd.associativity_lemma (list a) (append #a) ==
+                       (forall (x y z : list a) . (x @ y) @ z == x @ (y @ z)))
+                by T.(norm [delta]; trefl ());
+            introduce forall (x y z : list a) . x @ (y @ z) == (x @ y) @ z
+                 with append_assoc x y z);
+  Mnd.intro_monoid (list a) [] (append #a)
+
+
+let rec permutation_t_sym #a l0 l1 (p : permutation_t #a l0 l1)
+  : Tot (permutation_t #a l1 l0)
+        (decreases p)
+  = match p with
+    | Perm_refl l -> Perm_refl l
+    | Perm_swap l0 x y l1 -> Perm_swap l0 y x l1
+    | Perm_trans l0 l1 l2 p0 p1 -> Perm_trans l2 l1 l0 (permutation_t_sym _ _ p1) (permutation_t_sym _ _ p0)
+
+let rec permutation_t_append (#a : Type) (pre l0 l1 sfx : list a) (p : permutation_t l0 l1)
+  : Tot (permutation_t (pre @ l0 @ sfx) (pre @ l1 @ sfx))
+        (decreases p)
+  = match p with
+    | Perm_swap l0 x y l1 ->
+                introduce forall x y . (pre @ l0) @ x :: y :: (l1 @ sfx) == pre @ (l0 @ x :: y :: l1) @ sfx
+                  with calc ( == ) {
+                    (pre @ l0) @ x :: y :: (l1 @ sfx);
+                  == {append_assoc pre l0 (x :: y :: (l1 @ sfx))}
+                    pre @ (l0 @ [x; y] @ (l1 @ sfx));
+                  == {append_assoc l0 [x; y] (l1 @ sfx)}
+                    pre @ ((l0 @ [x; y]) @ (l1 @ sfx));
+                  == {append_assoc (l0@[x; y]) l1 sfx}
+                    pre @ (((l0 @ [x; y]) @ l1) @ sfx);
+                  == {append_assoc l0 [x; y] l1}
+                    pre @ (l0 @ x :: y :: l1) @ sfx;
+                  };
+                Perm_swap (pre @ l0) x y (l1 @ sfx)
+    | Perm_refl l0 -> Perm_refl _
+    | Perm_trans l0 l1 l2 p0 p1 ->
+                 Perm_trans _ _ _ (permutation_t_append pre l0 l1 sfx p0)
+                                  (permutation_t_append pre l1 l2 sfx p1)
+
+let rec permutation_t_cons_snoc #a x l
+  : Tot (permutation_t #a (x :: l) (snoc (l,x)))
+        (decreases l)
+  = match l with
+    | [] -> Perm_refl _
+    | hd :: tl ->
+      Perm_trans _ _ _ (Perm_swap [] x hd tl)
+                       (permutation_t_append [hd] (x :: tl) (snoc (tl,x)) []
+                         (permutation_t_cons_snoc #a x tl))
+        
+let rec permutation_t_reverse #a l
+  : Tot (permutation_t #a l (reverse l))
+        (decreases l)
+  = match l with
+    | [] -> Perm_refl _
+    | hd :: tl ->
+      Perm_trans _ _ _ (permutation_t_cons_snoc hd tl)
+                       (permutation_t_append [] tl (reverse tl) [hd]
+                         (permutation_t_reverse tl))
+
+(* [g_fold_right] *)
+
+let rec fold_right_gtot_append #a #b l0 l1 f x
+  : Lemma (ensures fold_right_gtot #a #b (l0@l1) f x == fold_right_gtot l0 f (fold_right_gtot l1 f x))
+          (decreases l0)
+  = match l0 with
+    | [] -> ()
+    | hd :: tl -> fold_right_gtot_append tl l1 f x
+
+let fold_right_gtot_f_comm #a #b (f : a -> b -> GTot b) : prop =
+  forall (x0 x1 : a) (y : b) . f x0 (f x1 y) == f x1 (f x0 y)
+
+let rec fold_right_gtot_comm_permutation_t #a #b l0 l1 f x (p : permutation_t l0 l1)
+  : Lemma (requires fold_right_gtot_f_comm #a #b f)
+          (ensures fold_right_gtot l0 f x == fold_right_gtot l1 f x)
+          (decreases p)
+  = match p with
+    | Perm_refl _ -> ()
+    | Perm_swap l0 x0 x1 l1 ->
+                fold_right_gtot_append l0 (x0 :: x1 :: l1) f x;
+                fold_right_gtot_append l0 (x1 :: x0 :: l1) f x
+    | Perm_trans l0 l1 l2 p0 p1 ->
+                fold_right_gtot_comm_permutation_t l0 l1 f x p0;
+                fold_right_gtot_comm_permutation_t l1 l2 f x p1
