Learn.LowStar.List.fst
@@ -33,11 +33,16 @@ type list_seg (a : Type0) = {
 
 let list_nil (a : Type0) : Type = sg:list_seg a{sg.exit == B.null}
 
+
 unfold let sg_v (#a : Type0) (sg : list_seg a) : Tot (list a)
   = L.map snd sg.segment
 
 unfold let sg_length (#a : Type0) (sg : list_seg a) : Tot nat
   = L.length sg.segment
+
+let sg_cell (#a : Type0) (sg : list_seg a) (i : nat)
+  : Ghost (B.pointer (cell a)) (requires i < sg_length sg) (ensures fun _ -> True)
+  = (L.index sg.segment i)._1
 
 let entry (#a : Type0) (sg : list_seg a) : Tot (t a)
   = if Nil? sg.segment then sg.exit else (L.hd sg.segment)._1
@@ -49,6 +54,7 @@ unfold let tail_seg (#a : Type0) (sg : list_seg a)
 unfold let append_seg (#a : Type0) (sg0 sg1 : list_seg a) : Tot (list_seg a)
   = { segment = L.(sg0.segment @ sg1.segment);
       exit    = sg1.exit }
+
 
 let rec loc_seg (#a : Type) (sg : list_seg a) : GTot M.loc
   (decreases sg.segment)
@@ -70,6 +76,7 @@ let rec live_seg (#a : Type) (h : HS.mem) (sg : list_seg a) : Tot prop
     | hd :: tl -> let sg' = tail_seg sg in 
                B.live h hd._1 /\ B.deref h hd._1 == {next = entry sg'; data = hd._2} /\ live_seg h sg'
 
+
 let rec loc_seg_live_in (#a : Type) (h : HS.mem) (sg : list_seg a)
   : Lemma (requires live_seg h sg) (ensures B.loc_in (loc_seg sg) h)
           (decreases sg.segment)
@@ -78,8 +85,28 @@ let rec loc_seg_live_in (#a : Type) (h : HS.mem) (sg : list_seg a)
     | [] -> ()
     | _ :: _ -> loc_seg_live_in h (tail_seg sg)
 
+let rec loc_seg_includes_cell (#a : Type) (sg : list_seg a) (i : nat)
+  : Lemma (requires  i < sg_length sg)
+          (ensures   M.(loc_includes (loc_seg sg) (loc_buffer (sg_cell sg i))))
+          (decreases i)
+          [SMTPat (sg_cell sg i); SMTPat (loc_seg sg)]
+  = if i = 0 then () else loc_seg_includes_cell (tail_seg sg) (i - 1)
+
+let loc_union_comm12 (s0 s1 s2 : M.loc)
+  : Lemma M.(loc_union s0 (loc_union s1 s2) == loc_union s1 (loc_union s0 s2))
+  = M.(loc_union_assoc s0 s1 s2; loc_union_comm s0 s1; loc_union_assoc s1 s0 s2)
+
+let loc_seg_fold_f #a (c : B.pointer (cell a) & a) : M.loc -> GTot M.loc
+  = M.(loc_union (loc_buffer c._1))
+
+let loc_seg_fold_f_comm a :
+  Lemma (ensures Ll.fold_right_gtot_f_comm (loc_seg_fold_f #a))
+  = let f = loc_seg_fold_f #a in
+    introduce forall x0 x1 y . f x0 (f x1 y) == f x1 (f x0 y)
+      with loc_union_comm12 M.(loc_buffer x0._1) M.(loc_buffer x1._1) y
+
 let rec loc_seg_fold (#a : Type) (sg : list_seg a)
-  : Lemma (ensures loc_seg sg == L.fold_right_gtot sg.segment (fun c -> M.(loc_union (loc_buffer c._1))) M.loc_none)
+  : Lemma (ensures loc_seg sg == L.fold_right_gtot sg.segment loc_seg_fold_f M.loc_none)
           (decreases sg.segment)
   = match sg.segment with
     | [] -> ()
@@ -117,19 +144,12 @@ let rec append_seg_live (#a : Type) (h : HS.mem) (sg0 sg1 : list_seg a)
     | [] -> ()
     | _ :: _ -> append_seg_live h (tail_seg sg0) sg1
 
-(*
-let rec loc_disjoint_seg_for_all (#a : Type) (loc : M.loc) (sg : list_seg a)
-  : Lemma (ensures M.loc_disjoint loc (loc_seg sg)
-                   <==> Ll.for_allP (M.loc_disjoint loc)
-                                  (L.map_gtot (fun (c : B.pointer (cell a) & a) -> M.loc_buffer c._1) sg.segment))
-  = admit ()
-*)
-
 let rec frame (#a : Type) (h0 h1 : HS.mem) (sg : list_seg a) (r : B.loc)
   : Lemma (requires live_seg h0 sg /\ M.(modifies r h0 h1 /\ loc_disjoint r (loc_seg sg)))
           (ensures  live_seg h1 sg)
           (decreases sg.segment)
-    [SMTPat (live_seg h0 sg); SMTPat (M.modifies r h0 h1)]
+    [SMTPat (live_seg #a h0 sg); SMTPat (M.modifies r h0 h1)]
+    (* or [SMTPat (M.modifies r h0 h1); SMTPat (live_seg #a h1 sg)] ? *)
   = match sg.segment with
     | [] -> ()
     | hd :: tl -> frame h0 h1 (tail_seg sg) r
@@ -143,6 +163,161 @@ let null_is_empty (#a : Type0) (h : HS.mem) (sg : list_seg a)
           (ensures  sg == empty_list a)
   = match sg.segment with
     | [] -> ()
+
+
+
+
+(* [reverse] *)
+
+let reverse_seg (#a : Type) (sg : list_seg a) =
+  { segment = L.rev sg.segment; exit = B.null }
+
+let reverse_seg_loc (#a : Type) (sg : list_seg a)
+  : Lemma (ensures loc_seg (reverse_seg sg) == loc_seg sg)
+    [SMTPat (loc_seg (reverse_seg sg))]
+  =
+    loc_seg_fold (reverse_seg sg);
+    loc_seg_fold sg;
+    loc_seg_fold_f_comm a;
+    Ll.fold_right_gtot_comm_permutation_t _ _ (loc_seg_fold_f #a)
+                 M.loc_none (Ll.permutation_t_reverse sg.segment);
+    Ll.rev_reverse sg.segment
+
+let reverse_ct_hyps #a
+      (sg : list_nil a) (lloc : M.loc)
+      (it_f it_r : B.pointer (t a)) (sgs : B.pointer (G.erased (list_nil a & list_nil a)))
+  = wf_seg sg /\
+  M.(let b_it_f = loc_buffer it_f in
+     let b_it_r = loc_buffer it_r in
+     let b_sgs  = loc_buffer sgs  in
+    loc_includes lloc (loc_union b_it_f (loc_union b_it_r b_sgs)) /\
+    loc_disjoint b_it_f b_it_r /\ loc_disjoint b_it_f b_sgs /\
+    loc_disjoint b_it_r b_sgs /\
+    M.loc_disjoint lloc (loc_seg sg))
+
+let reverse_ct_inv #a
+      (sg : list_nil a) (lloc : M.loc)
+      (it_f it_r : B.pointer (t a)) (sgs : B.pointer (G.erased (list_nil a & list_nil a)))
+      (h0 h : HS.mem)
+  =
+    M.(modifies (loc_union lloc (loc_seg sg)) h0 h) /\
+    B.(live h it_f /\ live h it_r /\ live h sgs) /\
+   (let p_f = B.deref h it_f in
+    let p_r = B.deref h it_r in
+    let (sg_f, sg_r) = G.reveal (B.deref h sgs) in
+    p_f == entry sg_f /\ p_r == entry sg_r /\
+    live_seg h sg_f /\ live_seg h sg_r /\
+    sg.segment == L.rev_acc sg_r.segment sg_f.segment /\
+    M.(loc_includes (loc_seg sg) (loc_seg sg_f) /\
+       loc_disjoint (loc_union lloc (loc_seg sg_f)) (loc_seg sg_r) /\
+       wf_seg sg_f))
+
+let reverse_ct_inv_test #a sg lloc it_f it_r
+       (sgs : B.pointer (G.erased (list_nil a & list_nil a))) h0 (b:bool) h
+  = reverse_ct_inv #a sg lloc it_f it_r sgs h0 h /\
+    (Cons? (G.reveal (B.deref h sgs))._1.segment <==> b)
+
+inline_for_extraction
+let reverse_loop_test #a
+      (sg : G.erased (list_nil a)) (lloc : G.erased M.loc)
+      (it_f it_r : B.pointer (t a)) (sgs : B.pointer (G.erased (list_nil a & list_nil a)))
+      h0 ()
+  : Stack bool
+     (requires fun h     -> reverse_ct_inv  sg lloc it_f it_r sgs h0 h)
+     (ensures  fun _ b h -> reverse_ct_inv_test sg lloc it_f it_r sgs h0 b h)
+  =
+    not (B.is_null it_f.(0ul)) 
+
+(* permet de forcer une preuve de [M.modifies] par transitivité *)
+noeq type mod_seq (#mod : M.loc) : HS.mem -> HS.mem -> Type =
+  | MNil  : h : HS.mem -> mod_seq #mod h h
+  | MCons : h0 : HS.mem -> #h1 : HS.mem -> #h2 : HS.mem ->
+               #squash (M.modifies mod h0 h1) -> mod_seq #mod h1 h2 -> mod_seq #mod h0 h2
+
+let rec mod_of_seq (mod : M.loc) (#h0 #h1 : HS.mem) (sq : mod_seq #mod h0 h1)
+  : Lemma (ensures M.modifies mod h0 h1) (decreases sq)
+  = match sq with
+    | MNil _ -> ()
+    | MCons _ sq -> mod_of_seq mod sq
+
+#push-options "--fuel 1 --ifuel 1"
+(* live_seg pose problème sans ces options *)
+
+inline_for_extraction
+let reverse_loop_body #a
+      (sg : G.erased (list_nil a)) (lloc : G.erased M.loc)
+      (it_f it_r : B.pointer (t a)) (sgs : B.pointer (G.erased (list_nil a & list_nil a)))
+      h0 ()
+  : Stack unit
+     (requires fun h      -> reverse_ct_hyps sg lloc it_f it_r sgs /\
+                          reverse_ct_inv  sg lloc it_f it_r sgs h0 h /\
+                          Cons? (G.reveal (B.deref h sgs))._1.segment)
+     (ensures  fun _ () h -> reverse_ct_inv  sg lloc it_f it_r sgs h0 h)
+  =
+      let h = ST.get () in
+      let sg_f = G.hide ((G.reveal (B.deref h sgs))._1) in
+      let sg_r = G.hide ((G.reveal (B.deref h sgs))._2) in
+    let cell : B.pointer (cell a) = it_f.(0ul) in
+    it_f.(0ul) <- (cell.(0ul)).next;
+      let h_1 = ST.get () in
+    cell.(0ul) <- {cell.(0ul) with next = it_r.(0ul)};
+      let h_2 = ST.get () in
+    it_r.(0ul) <- cell;
+      let h_3 = ST.get () in
+      sgs.(0ul)  <- G.hide (tail_seg sg_f, {segment = L.hd sg_f.segment :: sg_r.segment; exit = B.null});
+      let h' = ST.get () in
+      mod_of_seq M.(loc_union lloc (loc_buffer cell))
+                   (MCons h (MCons h_1 (MCons h_2 (MCons h_3 (MNil h')))));
+      mod_of_seq M.(loc_union lloc (loc_seg sg))
+                   (MCons h0 (MCons h (MNil h')));
+      let sg_f' = G.hide (G.reveal (B.deref h' sgs))._1 in
+      let sg_r' = G.hide (G.reveal (B.deref h' sgs))._2 in
+      assert (sg.segment == L.rev_acc sg_r'.segment sg_f'.segment)
+
+let reverse (#a : Type) (p : t a) (sg : G.erased (list_nil a))
+  : Stack (t a) (requires fun h0 -> live_seg h0 sg /\
+                                 wf_seg sg /\
+                                 p == entry sg)
+                (ensures fun h0 p' h1 -> M.modifies (loc_seg sg) h0 h1 /\
+                                (let sg' = reverse_seg sg in
+                                 live_seg h1 sg' /\
+                                 p' == entry sg'))
+  =
+      let h00 = ST.get () in
+    push_frame ();
+      let h01 = ST.get () in
+    let it_f = B.alloca #(t a) p      1ul in
+    let it_r = B.alloca #(t a) B.null 1ul in
+      let sgs  = B.alloca #(G.erased (list_nil a & list_nil a))
+                           (G.reveal sg, empty_list a) 1ul in
+      let h0 = ST.get () in
+      let lloc = G.hide (M.loc_region_only true (HS.get_tip h0)) in
+    assert (reverse_ct_hyps sg lloc it_f it_r sgs);
+    assert (reverse_ct_inv  sg lloc it_f it_r sgs h0 h0);
+    C.Loops.while #(reverse_ct_inv sg lloc it_f it_r sgs h0)
+                  #(reverse_ct_inv_test sg lloc it_f it_r sgs h0)
+                   (reverse_loop_test sg lloc it_f it_r sgs h0)
+                   (reverse_loop_body sg lloc it_f it_r sgs h0);
+    let rt = it_r.(0ul) in
+      let h1 = ST.get () in
+      let sg_f = G.hide ((G.reveal (B.deref h1 sgs))._1) in
+      let sg_r = G.hide ((G.reveal (B.deref h1 sgs))._2) in
+      assert (reverse_ct_inv  sg lloc it_f it_r sgs h0 h1);
+      U.assert_by (G.reveal sg_r == reverse_seg sg) (fun () ->
+        assert (G.reveal sg_f == empty_list a);
+        assert (sg.segment == L.rev sg_r.segment);
+        L.rev_involutive (sg_r.segment));
+      assert (rt == entry sg_r);
+      assert (live_seg h1 sg_r);
+      assert M.(modifies (loc_union lloc (loc_seg sg)) h0 h1);
+      assert M.(modifies loc_none h01 h0);
+      assert M.(modifies (loc_union (loc_all_regions_from false (HS.get_tip h1)) (loc_seg sg)) h01 h1);
+    pop_frame ();
+      let h1' = ST.get () in
+      M.modifies_fresh_frame_popped h00 h01 (loc_seg sg) h1 h1'; (* appel explicit nécessaire *)
+    rt
+
+#pop-options
 
 
 (* --- length --- *)
@@ -176,18 +351,19 @@ let length_loop_body a (l:Ghost.erased nat) h0 r
     (p     : B.pointer (t a))
     (seg   : B.pointer (Ghost.erased (list_nil a)))
     (count : B.pointer (U32.t))
-  (() : squash M.(loc_disjoint (loc_buffer p)   (loc_buffer seg) /\
+  (hyp0 : squash M.(loc_disjoint (loc_buffer p)   (loc_buffer seg) /\
                   loc_disjoint (loc_buffer p)   (loc_buffer count) /\
                   loc_disjoint (loc_buffer seg) (loc_buffer count) /\
                   loc_includes (loc_region_only true r)
                      (loc_union (loc_buffer p) (loc_union (loc_buffer seg) (loc_buffer count)))))
-  (() : squash (l <= FStar.UInt.max_int U32.n))
-  : unit -> Stack unit (requires fun h -> length_test_inv a l h0 r p seg count true h)
-                      (ensures fun _ () h -> length_inv a l h0 r p seg count h)
-  = fun () -> p.(0ul) <- (p.(0ul).(0ul)).next;
-           let seg0 = seg.(0ul) in
-           seg.(0ul) <- Ghost.hide (tail_seg seg0);
-           count.(0ul) <- U32.(count.(0ul) +^ 1ul)
+  (hyp1 : squash (l <= FStar.UInt.max_int U32.n))
+  () : Stack unit (requires fun h     -> length_test_inv a l h0 r p seg count true h)
+                  (ensures fun _ () h -> length_inv a l h0 r p seg count h)
+  =
+      let seg0 = seg.(0ul) in
+    p.(0ul) <- (p.(0ul).(0ul)).next;
+      seg.(0ul) <- Ghost.hide (tail_seg seg0);
+    count.(0ul) <- U32.(count.(0ul) +^ 1ul)
 
 let length_loop (#a : Type0) (p : t a) (sg : G.erased (list_nil a){p == entry sg}):
   Stack U32.t
@@ -244,9 +420,11 @@ let rec initi (#a : Type0) (r : HS.rid) (lb ub : U32.t)
          sg_v sg == Ll.initi (U32.v lb) (U32.v ub) fg)
   = if U32.(lb <^ ub) then begin
        let fg' : G.erased ((i:nat{U32.v lb + 1 <= i /\ i < U32.v ub}) -> Tot a) =
-         let fg' = G.reveal fg in G.hide fg'  in
+         let fg' = G.reveal fg in G.hide fg' in
        let (|p', sg'|) = initi r U32.(lb +^ 1ul) ub fg' f in
        let p = B.malloc r ({ data = f lb; next = p' }) 1ul in
+         let h' = ST.get() in
+         assert (live_seg h' (push_seg p (f lb) sg'));
        (| p, G.hide (push_seg p (f lb) sg')|)
     end else
        (| B.null, G.hide (empty_list a) |)
@@ -301,10 +479,6 @@ let index_loop (#a : Type0) (p : t a) (sg : G.erased (list_seg a){p == entry sg}
 
 (* version fonctionnelle *)
 
-let loc_union_comm12 (s0 s1 s2 : M.loc)
-  : Lemma M.(loc_union s0 (loc_union s1 s2) == loc_union s1 (loc_union s0 s2))
-  = M.(loc_union_assoc s0 s1 s2; loc_union_comm s0 s1; loc_union_assoc s1 s0 s2)
-
 let rec insert_seg_loc (#a : Type) (i : nat) (x : B.pointer (cell a) & a) (sg : list_seg a)
   : Lemma (requires i <= sg_length sg)
           (ensures loc_seg ({sg with segment = Ll.insert i x sg.segment})
@@ -330,6 +504,7 @@ let insert_post (#a : Type) (r : HS.rid) (i : nat) (x : a) (sg : list_seg a)
   = M.(modifies mod h0 h1 /\
        fresh_loc (loc_buffer p_f) h0 h1 /\
        loc_includes (loc_region_only true r) (loc_buffer p_f)) /\
+    B.freeable p_f /\
    (let sg' = {sg with segment = Ll.insert i (p_f, x) sg.segment} in
     live_seg h1 sg' /\ wf_seg sg' /\
     p1 == entry sg')
@@ -375,7 +550,7 @@ let insert (#a : Type) (r : HS.rid) (i : U32.t) (x : a) (p : t a) (sg : G.erased
 let insert_loop_pre (#a : Type) (r : HS.rid) (x : a)
                     (l_p : B.pointer (t a)) (l_sg : B.pointer (G.erased (list_seg a)))
                     (i : nat) (h0 : HS.mem) : Tot prop
-  = M.(live h0 l_p /\live h0 l_sg /\ loc_disjoint (loc_buffer l_p) (loc_buffer l_sg)) /\
+  = M.(live h0 l_p /\ live h0 l_sg /\ loc_disjoint (loc_buffer l_p) (loc_buffer l_sg)) /\
   ( let p = B.deref h0 l_p in let sg = B.deref h0 l_sg in
     M.(loc_disjoint (loc_union (loc_buffer l_p) (loc_buffer l_sg)) (loc_seg sg)) /\
     insert_pre r i h0 p sg)
@@ -486,12 +661,11 @@ let insert_loop_lemma1 #a r i (x : a) p sg (p_f : B.pointer (cell a)) (l_locals 
     assert M.(modifies (loc_union l_locals (loc_seg sg)) h2 h3);
     M.modifies_fresh_frame_popped h0 h1 (loc_seg sg) h3 h4;
     assert M.(modifies (loc_seg sg) h0 h4);
-
-    assert M.(fresh_loc (loc_buffer p_f) h2 h3);
-    assert M.(fresh_loc (loc_buffer p_f) h0 h4);
-
+ 
     assert (live_seg h3 sg');
-    assert (live_seg h4 sg')
+    assert (live_seg h4 sg');
+
+    assert M.(fresh_loc (loc_buffer p_f) h0 h4)
 
 inline_for_extraction
 let insert_loop0 (#a : Type) (r : HS.rid) (i : U32.t) (x : a) (p : t a) (sg : G.erased (list_seg a))
@@ -539,6 +713,240 @@ let insert_loop (#a : Type) (r : HS.rid) (i : U32.t) (x : a) (p : t a) (sg : G.e
     rt
 
 
+(* [forward] *)
+
+let splitAt_seg (#a:Type) (n:nat) (sg:list_seg a) : Tot (list_seg a & list_seg a) =
+  let l0, l1 = L.splitAt n sg.segment in
+  let sg1 = {segment = l1; exit = sg.exit} in
+  {segment = l0; exit = entry sg1}, sg1
+
+unfold let splitAt_seg_bd (#a:Type) (n:nat) (sg:list_seg a)
+  : Pure (list_seg a & list_seg a)
+         (requires n <= sg_length sg)
+         (ensures fun (sg0,sg1) -> sg_length sg0 = n /\ sg_length sg1 = sg_length sg - n)
+  = L.splitAt_length n sg.segment;
+    splitAt_seg n sg
+
+let splitAt_append_seg (#a:Type) (n:nat) (sg:list_seg a)
+  : Lemma (let sg0,sg1 = splitAt_seg n sg in append_seg sg0 sg1 == sg)
+  = Ll.lemma_splitAt_append n sg.segment
+
+let splitAt_seg_wf (#a : Type) (n:nat) (sg : list_seg a)
+  : Lemma (let sg0,sg1 = splitAt_seg n sg in
+          (wf_seg sg <==> wf_seg sg0 /\ wf_seg sg1 /\ M.loc_disjoint (loc_seg sg0) (loc_seg sg1)))
+  = splitAt_append_seg n sg
+
+let splitAt_seg_live (#a:Type) (n:nat) (h : HS.mem) (sg:list_seg a)
+  : Lemma (let sg0,sg1 = splitAt_seg n sg in
+          (live_seg h sg <==> live_seg h sg0 /\ live_seg h sg1))
+  = splitAt_append_seg n sg
+
+let splitAt_seg_entry (#a:Type) (n:nat) (sg:list_seg a)
+  : Lemma (entry (splitAt_seg n sg)._1 == entry sg)
+  = ()
+
+let forward_inv (#a : Type) (sg : list_seg a) (h0 : HS.mem)
+                            (i : nat)  (p : t a) (h1 : HS.mem)
+  : Tot prop
+  = M.(modifies loc_none h0 h1) /\ p == entry (splitAt_seg i sg)._2
+
+let rec splitAt_next (#a : Type) (i : nat) (sg : list_seg a)
+  : Lemma (requires i < sg_length sg)
+          (ensures  (splitAt_seg_bd (i + 1) sg)._2 == tail_seg (splitAt_seg_bd i sg)._2)
+          (decreases i)
+  = if i = 0 then () else splitAt_next (i - 1) (tail_seg sg)
+
+let rec splitAt_next_live (#a : Type) (i : nat) (sg : list_seg a) (h : HS.mem)
+  : Lemma (requires live_seg h sg /\ i < sg_length sg)
+          (ensures (let sg1 = (splitAt_seg_bd i sg)._2 in
+                    let ptr = entry sg1 in
+                    Cons? sg1.segment /\
+                    (splitAt_seg_bd (i+1) sg)._2 == tail_seg sg1 /\
+                    ~(B.g_is_null ptr) /\ B.live h ptr /\
+                    (B.deref h ptr).next == entry (tail_seg sg1)))
+          (decreases i)
+  = splitAt_seg_live i h sg;
+    if i = 0 then ()
+    else splitAt_next_live (i-1) (tail_seg sg) h
+
+inline_for_extraction
+let forward (#a : Type) (i : U32.t) (p : t a) (sg : G.erased (list_seg a))
+  : Stack (t a) (requires fun h0    -> U32.v i <= sg_length sg /\
+                                    live_seg h0 sg /\
+                                    p == entry sg)
+             (ensures  fun h0 p' h1 -> M.(modifies loc_none h0 h1) /\
+                                    p' == entry (splitAt_seg_bd (U32.v i) sg)._2)
+  = push_frame ();
+    let l_p = B.alloca #(t a) p 1ul in
+    let h0 = ST.get () in
+    C.Loops.for 0ul i (fun h1 j -> M.(modifies (loc_buffer l_p) h0 h1) /\
+                                B.live h1 l_p /\
+                                B.deref h1 l_p == entry (splitAt_seg j sg)._2)
+                      (fun j -> let h1 = ST.get () in
+                             splitAt_next_live (U32.v j) sg h1;
+                             l_p.(0ul) <- (l_p.(0ul).(0ul)).next);
+    let rt = l_p.(0ul) in
+    pop_frame ();
+    rt
+
+(* [set] *)
+
+let set_seg (#a : Type) (i : nat) (x : a) (sg : list_seg a)
+  : Pure (list_seg a) (requires i < sg_length sg) (ensures fun sg' -> sg_length sg' = sg_length sg)
+  = { sg with segment = Ll.map_index i (fun (c, _) -> (c, x)) sg.segment }
+
+let rec set_seg_splitAt (#a : Type) (i j : nat) (x : a) (sg : list_seg a)
+  : Lemma (requires i + j < sg_length sg)
+          (ensures  set_seg (i + j) x sg
+                    == (let sg0,sg1 = splitAt_seg_bd i sg in
+                        append_seg sg0 (set_seg j x sg1)))
+          (decreases i)
+  = if i = 0 then ()
+    else (set_seg_splitAt (i-1) j x (tail_seg sg);
+          L.splitAt_length i sg.segment)
+
+let set (#a : Type) (i : U32.t) (x : a) (p : t a) (sg : G.erased (list_seg a))
+  : Stack unit (requires fun h0      -> U32.v i < sg_length sg /\
+                                     live_seg h0 sg /\ wf_seg sg /\
+                                     p == entry sg)
+               (ensures fun h0 () h1 -> M.(modifies (loc_buffer (sg_cell sg (U32.v i))) h0 h1) /\
+                                      live_seg h1 (set_seg (U32.v i) x sg))
+  =
+    let p' = forward i p sg in
+      let h0 = ST.get () in
+      let vi = U32.v i   in
+      let sg0 = G.hide (splitAt_seg vi sg)._1 in
+      let sg1 = G.hide (splitAt_seg vi sg)._2 in
+      splitAt_seg_wf vi sg;
+      splitAt_seg_live vi h0 sg;
+      L.splitAt_length vi sg.segment;
+      L.lemma_splitAt_reindex_right vi sg.segment 0;
+      assert (live_seg h0 sg1);
+    p'.(0ul) <- { p'.(0ul) with data = x };
+      let h1 = ST.get () in
+      U.assert_by (live_seg h1 (append_seg sg0 (set_seg 0 x sg1))) (fun () ->
+          assert (live_seg h1 (set_seg 0 x sg1));
+          assert (live_seg h1 sg0));
+      set_seg_splitAt (U32.v i) 0 x sg
+
+(* [last] *)
+
+inline_for_extraction
+let sg_next (#a : Type) (p : t a) (sg : G.erased (list_seg a))
+  : Stack (t a) (requires fun h0       -> live_seg h0 sg /\ p == entry sg /\ Cons? sg.segment)
+                (ensures  fun h0 p' h1 -> M.(modifies loc_none h0 h1) /\
+                                       live_seg h1 (tail_seg sg) /\ p' == entry (tail_seg sg))
+  = (p.(0ul)).next
+
+let last_ct_locals #a (l_it : B.pointer (B.pointer (cell a))) (l_k  : B.pointer (G.erased nat))
+  : GTot M.loc =
+  M.(loc_union (loc_buffer l_it) (loc_buffer l_k))
+
+let last_ct_hyps #a (sg : list_nil a) c_h0 l_it l_k : prop =
+  M.(loc_disjoint (last_ct_locals l_it l_k) (loc_seg sg) /\
+     loc_disjoint (loc_buffer l_it) (loc_buffer l_k)) /\
+  live_seg c_h0 sg
+
+let last_loop_inv #a sg c_h0 (l_it : B.pointer (B.pointer (cell a))) (l_k  : B.pointer (G.erased nat))
+                  (h : HS.mem) : prop =
+  M.(modifies (loc_union (loc_buffer l_it) (loc_buffer l_k)) c_h0 h /\
+     live h l_it /\ live h l_k) /\
+ (let vit = B.deref h l_it in
+  let vk  = B.deref h l_k  in
+  vk < sg_length #a sg /\
+  vit == entry (splitAt_seg_bd vk sg)._2)
+
+
+let lemma_last_loop_inv_it_live #a (sg : list_nil a) c_h0
+             (l_it : B.pointer (B.pointer (cell a))) (l_k  : B.pointer (G.erased nat)) h
+  : Lemma (requires last_ct_hyps sg c_h0 l_it l_k /\ last_loop_inv sg c_h0 l_it l_k h)
+          (ensures (let sg1 = (splitAt_seg_bd (B.deref h l_k) sg)._2 in
+                    live_seg h sg1 /\ Cons? sg1.segment))
+  = let vk = B.deref h l_k in
+    assert (live_seg h sg);
+    splitAt_seg_live vk h sg
+
+inline_for_extraction
+let last_loop_body #a (sg : G.erased (list_nil a)) c_h0
+             (l_it : B.pointer (B.pointer (cell a))) (l_k  : B.pointer (G.erased nat)) ()
+  : Stack unit (requires fun h      -> last_ct_hyps sg c_h0 l_it l_k /\
+                                    last_loop_inv sg c_h0 l_it l_k h /\
+                                    ~B.(g_is_null (deref h (deref h l_it)).next))
+               (ensures  fun _ () h -> last_loop_inv sg c_h0 l_it l_k  h)
+  =
+      let h0  = ST.get () in
+      let k0  = B.deref h0 l_k in
+      let sg0 = G.hide ((splitAt_seg_bd k0 sg)._2) in
+      lemma_last_loop_inv_it_live sg c_h0 l_it l_k h0;
+    l_it.(0ul) <- sg_next (l_it.(0ul)) sg0; 
+    l_k.(0ul)  <- k0 + 1;
+      let h1  = ST.get () in
+      U.assert_by (tail_seg sg0 == (splitAt_seg (k0 + 1) sg)._2)
+                  (fun () -> splitAt_next k0 sg)
+
+let last (#a : Type) (p : t a) (sg : G.erased (list_nil a))
+  : Stack (t a) (requires fun h0      -> live_seg h0 sg /\
+                                      p == entry sg /\
+                                      sg_length sg > 0)
+                (ensures fun h0 p' h1 -> M.(modifies loc_none h0 h1) /\
+                                     (let sg' = (splitAt_seg_bd (sg_length sg - 1) sg)._2 in
+                                      p' == entry sg'))
+  =
+    push_frame ();
+    let it = B.alloca #(B.pointer (cell a)) p 1ul in
+    let k  = B.alloca #(G.erased nat) 0 1ul         in
+      let h0 = ST.get () in
+      assert (last_ct_hyps sg h0 it k);
+      let inv = last_loop_inv sg h0 it k in
+      let test_post (b : bool) (h : HS.mem) =
+        inv h /\ (B.(g_is_null (deref h (deref h it)).next) <==> not b)
+    in
+    let test () : Stack bool (requires fun h -> inv h) (ensures fun _ b h -> test_post b h)
+      = let h = ST.get () in lemma_last_loop_inv_it_live sg h0 it k h;
+        not (B.is_null (it.(0ul).(0ul)).next)
+    in
+    C.Loops.while #(fun h -> inv h) #test_post test (last_loop_body sg h0 it k);
+      let h1 = ST.get () in
+      lemma_last_loop_inv_it_live sg h0 it k h1;
+      assert (sg_length (splitAt_seg_bd (B.deref h1 k) sg)._2 == 1);
+      assert (G.reveal (B.deref h1 k) = sg_length sg - 1);
+    let rt = it.(0ul) in
+    pop_frame ();
+    rt
+
+(* [append] *)
+
+let append (#a : Type) (p0 : t a) (sg0 : G.erased (list_nil a)) (p1 : t a) (sg1 : G.erased (list_seg a))
+  : Stack (t a) (requires fun h0 -> live_seg h0 sg0 /\
+                                 wf_seg sg0 /\ M.loc_disjoint (loc_seg sg0) (loc_seg sg1) /\
+                                 p0 == entry sg0 /\
+                                 p1 == entry sg1)
+                (ensures fun h0 p h1 -> M.modifies (loc_seg sg0) h0 h1 /\
+                                   ( let sg = append_seg ({sg0 with exit = entry sg1}) sg1 in
+                                     p == entry sg /\
+                                    (live_seg h0 sg1 ==> live_seg h1 sg)))
+  =
+      let h00 = ST.get () in
+    if B.is_null p0 then p1
+    else begin
+      let p0_last = last p0 sg0 in
+        let h0 = ST.get () in
+        let sg00 = G.hide (splitAt_seg_bd (sg_length sg0 - 1) sg0)._1 in
+        let sg01 = G.hide (splitAt_seg_bd (sg_length sg0 - 1) sg0)._2 in
+        splitAt_append_seg (sg_length sg0 - 1) sg0;
+        splitAt_seg_live (sg_length sg0 - 1) h0 sg0;
+        splitAt_seg_wf   (sg_length sg0 - 1) sg0;
+        assert (p0_last == entry sg01);
+        assert (live_seg h0 sg01);
+        assert M.(loc_includes (loc_seg sg0) (loc_buffer (L.hd sg01.segment)._1));
+      p0_last.(0ul) <- { p0_last.(0ul) with next = p1 };
+        let h1 = ST.get () in
+        assert M.(modifies (loc_seg sg0) h0 h1);
+        assert (live_seg h1 sg00);
+        assert (live_seg h1 ({sg01 with exit = p1}));
+      p0
+    end
+
 (* ------------------------------------------------------------------------------------------- *)
 
 let length_loop_u32 = length_loop #U32.t
@@ -557,6 +965,16 @@ let index_loop_u32 = index_loop #U32.t
 let insert_u32 = insert #U32.t
 
 let insert_loop_u32 = insert_loop #U32.t
+
+let forward_u32 = forward #U32.t
+
+let set_u32 = set #U32.t
+
+let last_u32 = last #U32.t
+
+let append_u32 = append #U32.t
+
+let reverse_u32 = reverse #U32.t
 
 let test_for () : Stack unit (fun _ -> True) (fun _ _ _ -> True)
   =
